Run.thy
@@ -1,0 +1,32 @@
+theory Run
+  \<comment> \<open>Check Isabelle's "Theories" panel to see the progress on loading theories\<close>
+  imports
+    "VerIso/S2PL_Proof" \<comment> \<open>1.5 min\<close>
+    "VerIso/EP+_Proof" \<comment> \<open>12 min\<close>
+    "VerIso/Tapir_Falsification" \<comment> \<open>1.5 min\<close>
+begin
+
+text \<open>Please make sure "Proof state" is checked in Isabelle's "Output" tab.
+  - To see the lemmas or theorems listed below, place the cursor on them .
+  - To see the lemma statement in the original theory where it is proven, Ctrl + Click on its name. (Cmd + Click for mac users) \<close>
+
+text \<open>Section 4.2\<close>
+
+thm tpl_refines_sser \<comment> \<open>Theorem 3\<close>
+
+
+text \<open>Section 5.5.2\<close>
+
+thm lemma_5
+thm lemma_6
+
+thm Correctness_of_EPP \<comment> \<open>Theorem 4\<close>
+
+
+text \<open>Section 6.2\<close>
+
+thm tapir_refines_sser
+  \<comment> \<open>fails: checkout the proof state at line 486 (in Isabelle's "Output" tab)\<close>
+
+
+end
